Mark parsers erased in stateful validators

examples/kv_parsing/PureEncoder.fst
@@ -3,6 +3,7 @@ module PureEncoder
 open FStar.Seq
 module U16 = FStar.UInt16
 module U32 = FStar.UInt32
+module Cast = FStar.Int.Cast
 module List = FStar.List.Tot
 
 open KeyValue
@@ -13,7 +14,10 @@ open PureParser
 (* TODO: somewhat minor, but standardize on a name for these (writer, encoder,
 serializer, emitter) *)
 
-assume val u16_to_be: U16.t -> b:bytes{length b == 2}
+val u16_to_be: U16.t -> b:bytes{length b == 2}
+let u16_to_be (n:U16.t) = create 1 (Cast.uint16_to_uint8 (U16.shift_right n 8ul)) `append`
+                          create 1 (Cast.uint16_to_uint8 (U16.rem n 256us))
+
 assume val u32_to_be: U32.t -> b:bytes{length b == 4}
 
 let encode_u16_array (len:U16.t) (b:bytes{length b == U16.v len}) : bytes =
